AP/AP/Defense/Edge/WF.lean
@@ -4,11 +4,11 @@ namespace AP.Edge
 
 variable {e e₁ e₂ : Edge}
 
-def cnd (e : Edge) (s : State) : Prop :=
+def cnd₀ (s : State) : Prop :=
   let pa := s.aPos
-  let p₀ := e.getBorderPoint₀ pa
-  let get := e.getBorderPoints pa
-  match e.dist pa with
+  let p₀ := edge₀.getBorderPoint₀ pa
+  let get := edge₀.getBorderPoints pa
+  match edge₀.dist pa with
   | 5 => p₀ ∈ s.taken
   | 4 => p₀ ∈ s.taken ∧ (get 1).any (· ∈ s.taken)
   | 3 => 2 ≤ (p₀ :: get 1).countP (· ∈ s.taken)
@@ -16,13 +16,63 @@ def cnd (e : Edge) (s : State) : Prop :=
   | 1 => (p₀ :: get 1).all (· ∈ s.taken)
   | d => 0 < d
 
-instance {e : Edge} {s} : Decidable # e.cnd s := by
-  simp [Edge.cnd]; split <;> all_goals infer_instance
+instance {s} : Decidable # cnd₀ s := by
+  simp [cnd₀]; split <;> all_goals infer_instance
 
-theorem wf_defense_of_down (h : e.dir = .down) : e.defense.WF := by
+theorem aPos_y_lt_zero_of_cnd₀ {s} (h : cnd₀ s) : s.aPos.y < 0 := by
+  simp [cnd₀, getBorderPoints, getBorderPoint₀, getBorderPoint, dist] at h ⊢
+  split at h <;> linarith
+
+theorem cnd₀_of_aPos_y_le_neg_6 {s} (h : s.aPos.y ≤ -6) : cnd₀ s := by
+  simp [cnd₀, getBorderPoints, getBorderPoint₀, getBorderPoint, dist] at h ⊢
+  split <;> linarith
+
+-- #check 0 #exit
+
+theorem cnd₀_simulate_of_aState {s} {a : AStrat} {d : DStrat} {n}
+[hs : AState s] [ha : a.WF] [hd : d.WF] (h : cnd₀ s) :
+cnd₀ # sys.simulate (Strat.f ⟨a, edge₀.defense.st d⟩) s n |>.1 := by
+  induction n using Nat.strong_induction_on
+  nm n ih
+  cases n; exact h; nm n
+  simp; split; exact h; nm x s₁ h₁; clear x
   sorry
 
 -- #check 0 #exit
+
+theorem edge₀_simulate_aPos_y_lt_zero_of_aState {s} {a : AStrat} {d : DStrat} {n}
+[hs : AState s] [ha : a.WF] [hd : d.WF] (h : s.aPos.y ≤ -6) :
+sys.simulate (Strat.f ⟨a, edge₀.defense.st d⟩) s n |>.1.aPos.y < 0 :=
+  aPos_y_lt_zero_of_cnd₀ # cnd₀_simulate_of_aState # cnd₀_of_aPos_y_le_neg_6 h
+
+theorem edge₀_simulate_aPos_y_lt_zero {s} {a : AStrat} {d : DStrat} {n}
+[hs : sys.WF s] [ha : a.WF] [hd : d.WF] (h : s.aPos.y ≤ -6) :
+sys.simulate (Strat.f ⟨a, edge₀.defense.st d⟩) s n |>.1.aPos.y < 0 := by
+  replace hs := s.aState_or_dState
+  rcases hs with hs | hs
+  · exact edge₀_simulate_aPos_y_lt_zero_of_aState h
+  cases n; simp; linarith; nm n
+  simp; split; simp; linarith; nm x s₁ h₁; clear x
+  have hs₁ := AState.of_tr h₁
+  apply edge₀_simulate_aPos_y_lt_zero_of_aState
+  rwa [DState.aPos_eq_of_tr h₁]
+
+theorem wf_defense_edge₀ : edge₀.defense.WF := by
+  use validTr_defense
+  intro s hs h a ha d hd n
+  simp [defense, points, memPoints]
+  apply edge₀_simulate_aPos_y_lt_zero
+  simp [defense, dist] at h
+  linarith
+
+theorem wf_defense_of_down (h : e.dir = .down) : e.defense.WF := by
+  have h₁ : edge₀.translate ⟨0, e.offset⟩ = e
+  · ext <;> simp [h]
+  rw [←h₁]
+  have H : Fact # edge₀.dir = .down; simp
+  rw [defense_translate_of_down]
+  have h₂ := wf_defense_edge₀
+  infer_instance
 
 theorem wf_defense_of_left (h : e.dir = .left) : e.defense.WF := by
   have h₁ : e.rotLeft.defense.WF
